Done DESCore_CORRECT

examples/Crypto/DES/desScript.sml
@@ -569,109 +569,122 @@ Overload FullDES = “DES 16”
 (*---------------------------------------------------------------------------*)
 
 (* The plaintext message halves and intermediate message halves m0 ~ m16 [3] *)
-Definition message_half_def :
-    message_half f ((u,v) :block) (ks :word48 list) n =
+Definition half_message_def :
+    half_message f ((u,v) :block) (ks :word48 list) n =
       if n = 0 then u
       else if n = 1 then v
-      else (message_half f (u,v) ks (n - 2)) ??
-           (f (message_half f (u,v) ks (n - 1)) (EL (n - 2) ks))
+      else (half_message f (u,v) ks (n - 2)) ??
+           (f (half_message f (u,v) ks (n - 1)) (EL (n - 2) ks))
 End
 
-Theorem message_half :
-    !f u v ks. message_half f (u,v) ks 0 = u /\
-               message_half f (u,v) ks 1 = v /\
+Theorem half_message :
+    !f u v ks. half_message f (u,v) ks 0 = u /\
+               half_message f (u,v) ks 1 = v /\
               (!n. 2 <= n ==>
-                   message_half f (u,v) ks n =
-                     (message_half f (u,v) ks (n - 2)) ??
-                     (f (message_half f (u,v) ks (n - 1)) (EL (n - 2) ks)))
+                   half_message f (u,v) ks n =
+                     (half_message f (u,v) ks (n - 2)) ??
+                     (f (half_message f (u,v) ks (n - 1)) (EL (n - 2) ks)))
 Proof
     rpt STRIP_TAC
- >- rw [Once message_half_def]
- >- rw [Once message_half_def]
+ >- rw [Once half_message_def]
+ >- rw [Once half_message_def]
  >> ‘n <> 0 /\ n <> 1’ by rw []
- >> GEN_REWRITE_TAC (RATOR_CONV o ONCE_DEPTH_CONV) empty_rewrites [message_half_def]
+ >> GEN_REWRITE_TAC (RATOR_CONV o ONCE_DEPTH_CONV) empty_rewrites [half_message_def]
  >> simp []
 QED
 
-Theorem message_half' :
-    !f uv ks. message_half f uv ks 0 = FST uv /\
-             message_half f uv ks 1 = SND uv /\
+Theorem half_message' :
+    !f uv ks. half_message f uv ks 0 = FST uv /\
+             half_message f uv ks 1 = SND uv /\
             (!n. 2 <= n ==>
-                 message_half f uv ks n =
-                  (message_half f uv ks (n - 2)) ??
-                  (f (message_half f uv ks (n - 1)) (EL (n - 2) ks)))
+                 half_message f uv ks n =
+                  (half_message f uv ks (n - 2)) ??
+                  (f (half_message f uv ks (n - 1)) (EL (n - 2) ks)))
 Proof
-    rpt GEN_TAC >> Cases_on ‘uv’ >> REWRITE_TAC [message_half]
+    rpt GEN_TAC >> Cases_on ‘uv’ >> REWRITE_TAC [half_message]
 QED
 
-(* This is message_half specialized for DES *)
-Overload M = “message_half RoundOp”
+(* This is half_message specialized for DES *)
+Overload M = “half_message RoundOp”
 
-Theorem Round_alt_message_half :
+Theorem Round_alt_half_message :
     !u v ks n. Round n ks (u,v) = (M (u,v) ks n, M (u,v) ks (SUC n))
 Proof
     NTAC 3 GEN_TAC
- >> Induct_on ‘n’ >- rw [Round_def, message_half]
+ >> Induct_on ‘n’ >- rw [Round_def, half_message]
  >> rw [Round_def]
  >> Q.ABBREV_TAC ‘m0 = M (u,v) ks n’
  >> Q.ABBREV_TAC ‘m1 = M (u,v) ks (SUC n)’
- >> simp [message_half, ARITH_PROVE “SUC (SUC n) - 2 = n”]
+ >> simp [half_message, ARITH_PROVE “SUC (SUC n) - 2 = n”]
 QED
 
-Theorem Round_alt_message_half' :
+Theorem Round_alt_half_message' :
     !ks uv n. Round n ks uv = (M uv ks n, M uv ks (SUC n))
 Proof
     rpt GEN_TAC >> Cases_on ‘uv’
- >> REWRITE_TAC [Round_alt_message_half]
+ >> REWRITE_TAC [Round_alt_half_message]
 QED
 
 (* FullDES can be expressed by just M16 and M17 *)
-Theorem FullDES_alt_message_half :
-    !ks plaintext. DESCore 16 ks plaintext =
-                   let uv = Split (IP plaintext) in
-                     IIP (Join (M uv ks 17, M uv ks 16))
+Theorem DESCore_alt_half_message :
+    !r ks plaintext. 0 < r ==>
+         DESCore r ks plaintext =
+           let uv = Split (IP plaintext) in
+             IIP (Join (M uv ks (SUC r), M uv ks r))
 Proof
-    rw [DESCore_alt, Round_alt_message_half', Swap_def]
+    rw [DESCore_alt, Round_alt_half_message', Swap_def]
+QED
+
+(* The key idea of this proof is from [3] based on half_message_def *)
+Theorem DESCore_CORRECT :
+    !keys r plaintext. LENGTH keys = r ==>
+       DESCore r (REVERSE keys) (DESCore r keys plaintext) = plaintext
+Proof
+    Q.X_GEN_TAC ‘ks’
+ >> rpt STRIP_TAC
+ >> Cases_on ‘r = 0’ >- rw [DESCore_0]
+ >> ‘0 < r’ by rw []
+ >> Know ‘DESCore r ks plaintext =
+          let uv = Split (IP plaintext) in
+            IIP (Join (M uv ks (SUC r), M uv ks r))’
+ >- rw [DESCore_alt_half_message]
+ >> Rewr'
+ >> rw [DESCore_def, IP_IIP_Inverse, Split_Join_Inverse,
+        RoundSwap_and_Round']
+ >> Q.ABBREV_TAC ‘uv = Split (IP plaintext)’
+ >> Q.ABBREV_TAC ‘r = LENGTH ks’
+ (* applying Round_def *)
+ >> Suff ‘Round r (REVERSE ks) (M uv ks (SUC r),M uv ks r) = (M uv ks 1,M uv ks 0)’
+ >- (Rewr' \\
+     rw [Abbr ‘uv’, half_message', Swap_def, Join_Split_Inverse, IIP_IP_Inverse])
+ >> Suff ‘!n. n <= r ==>
+              Round n (REVERSE ks) (M uv ks (SUC r),M uv ks r) =
+              (M uv ks (SUC r - n),M uv ks (r - n))’
+ >- (DISCH_THEN (MP_TAC o (Q.SPEC ‘r’)) >> rw [])
+ >> Induct_on ‘n’ >- rw [Round_def]
+ >> rw [Round_def]
+ >> Q.PAT_X_ASSUM ‘n <= r ==> _’ K_TAC
+ (* we have 3 numbers: ‘SUC r - n’, ‘r - n’ and ‘r - SUC n’, which is bigger? *)
+ >> Q.ABBREV_TAC ‘i = SUC r - n’
+ >> ‘r - n = i - 1’ by rw [Abbr ‘i’] >> POP_ORW
+ >> ‘r - SUC n = i - 2’ by rw [Abbr ‘i’] >> POP_ORW
+ >> ‘2 <= i’ by rw [Abbr ‘i’]
+ >> Know ‘M uv ks i =
+          M uv ks (i - 2) ?? (RoundOp (M uv ks (i - 1)) (EL (i - 2) ks))’
+ >- METIS_TAC [half_message']
+ >> Rewr'
+ >> Suff ‘EL n (REVERSE ks) = EL (i - 2) ks’ >- rw []
+ >> rw [Abbr ‘i’, Abbr ‘r’, EL_REVERSE]
+ >> Q.ABBREV_TAC ‘r = LENGTH ks’
+ >> Suff ‘PRE (r - n) = SUC r - (n + 2)’ >- Rewr
+ >> ARITH_TAC
 QED
 
 Theorem FullDES_CORRECT :
     !key plaintext. ((encrypt,decrypt) = FullDES key) ==>
                     (decrypt (encrypt plaintext) = plaintext)
 Proof
-    rw [DES_def]
- >> Q.ABBREV_TAC ‘ks = KS key 16’
- (* applying FullDES_alt_message_half *)
- >> Know ‘DESCore 16 ks plaintext =
-          let uv = Split (IP plaintext) in
-                     IIP (Join (M uv ks 17, M uv ks 16))’
- >- REWRITE_TAC [FullDES_alt_message_half]
- >> Rewr'
- >> rw [DESCore_def, IP_IIP_Inverse, Split_Join_Inverse,
-        RoundSwap_and_Round']
- >> Q.ABBREV_TAC ‘uv = Split (IP plaintext)’
- (* applying Round_def *)
- >> Suff ‘Round 16 (REVERSE ks) (M uv ks 17,M uv ks 16) = (M uv ks 1,M uv ks 0)’
- >- (Rewr' \\
-     rw [Abbr ‘uv’, message_half', Swap_def, Join_Split_Inverse, IIP_IP_Inverse])
- >> Suff ‘!n. n <= 16 ==>
-              Round n (REVERSE ks) (M uv ks 17,M uv ks 16) =
-              (M uv ks (17 - n),M uv ks (16 - n))’
- >- (DISCH_THEN (MP_TAC o (Q.SPEC ‘16’)) >> rw [])
- >> Induct_on ‘n’ >- rw [Round_def]
- >> rw [Round_def, ARITH_PROVE “16 - n = 17 - SUC n”]
- >> Q.PAT_X_ASSUM ‘n <= 16 ==> _’ K_TAC
- (* now we have 3 numbers: ‘17 - n’, ‘17 - SUC n’ and ‘17 - SUC (SUC n)’ *)
- >> Q.ABBREV_TAC ‘i = 17 - n’
- >> ‘17 - SUC n = i - 1’ by rw [Abbr ‘i’] >> POP_ORW
- >> ‘17 - SUC (SUC n) = i - 2’ by rw [Abbr ‘i’] >> POP_ORW
- >> ‘2 <= i’ by rw [Abbr ‘i’]
- >> Know ‘M uv ks i =
-          M uv ks (i - 2) ?? (RoundOp (M uv ks (i - 1)) (EL (i - 2) ks))’
- >- METIS_TAC [message_half']
- >> Rewr'
- >> Suff ‘EL n (REVERSE ks) = EL (i - 2) ks’ >- rw []
- >> rw [Abbr ‘ks’, Abbr ‘i’, EL_REVERSE, LENGTH_KS,
-        ARITH_PROVE “PRE (16 - n) = 15 - n”]
+    rw [DES_def, DESCore_CORRECT, LENGTH_KS]
 QED
 
 val _ = export_theory();
